code/Ch46.v
@@ -1,0 +1,707 @@
+Add LoadPath ".".
+Add LoadPath "/Users/sweirich/github/deepspec/metalib/" as Metalib.
+Require Import Metalib.Metatheory.
+
+Require Import systemt_inf.
+Require Import Ch9.
+
+(* This part of a development for chapter 46. I didn't have time to 
+   fill in all of the details, but it should make most of the 
+   chapter clear *)
+
+(* ------------ Observable equivalence -------------------- *)
+
+(* These are contexts --- basically we can consider them as terms 
+   with a "hole" in them. *)
+Inductive ctx : Set :=
+| ctx_top  : ctx    (* written  \circ in PFPL *)
+| ctx_s    : ctx -> ctx
+| ctx_rec1 : ctx -> exp -> atom -> atom -> typ -> exp -> ctx
+| ctx_rec2 : exp -> ctx -> atom -> atom -> typ -> exp -> ctx
+| ctx_rec3 : exp -> exp -> atom -> atom -> typ -> ctx -> ctx
+| ctx_abs  : typ -> atom -> ctx -> ctx
+| ctx_app1 : ctx -> exp -> ctx
+| ctx_app2 : exp -> ctx -> ctx.
+
+Notation close := close_exp_wrt_exp.
+
+(* Written C { e } in PFPL *)
+Fixpoint replace (C : ctx) (e : exp) :=
+  match C with
+  | ctx_top => e
+  | ctx_s C => s (replace C e)
+  | ctx_rec1 C e1 x y t e2 => rec (replace C e) e1 (close x (abs t (close y e2)))
+  | ctx_rec2 e0 C x y t e2 => rec e0 (replace C e) (close x (abs t (close y e2)))
+  | ctx_rec3 e0 e1 x y t C => rec e0 e1 (close x (abs t (close y (replace C e))))
+  | ctx_abs t x C => abs t (close x (replace C e))
+  | ctx_app1 C e2 => app (replace C e) e2
+  | ctx_app2 e1 C => app e1 (replace C e)
+  end.
+
+(* Written   C : G |> t ~> G' |> t' *)
+Inductive typing_ctx : ctx -> env -> typ -> env -> typ -> Prop :=
+| typing_ctx_top : forall G t, typing_ctx ctx_top G t G t
+| typing_ctx_s   : forall G t G' C,
+    typing_ctx C G t G' typ_nat ->
+    typing_ctx (ctx_s C) G t G' typ_nat
+| typing_ctx_rec1 : forall C G t G' t' x y e0 e1,
+    typing_ctx C G t G' typ_nat ->
+    typing G' e0 t' ->
+    value e1 -> 
+    typing ((y ~ t') ++ (x ~ typ_nat) ++ G') e1  t' ->
+    typing_ctx (ctx_rec1 C e0 x y t' e1) G t G' t'
+| typing_ctx_rec2 : forall C G t G' t' x y e0 e1,
+    typing G' e0 typ_nat ->
+    typing_ctx C G t G' t' ->
+    value e1 ->
+    typing ((y ~ t') ++ (x ~ typ_nat) ++ G') e1 t' ->
+    typing_ctx (ctx_rec2 e0 C x y t' e1) G t G' t'
+| typing_ctx_rec3 : forall C G t G' t' x y e0 e1,
+    typing G' e0 typ_nat ->
+    typing G' e1 t' ->
+    typing_ctx C G t ((y ~ t') ++ (x ~ typ_nat) ++ G') t' ->
+    typing_ctx (ctx_rec3 e0 e1 x y t' C) G t G' t'
+| typing_ctx_abs : forall C G G' t t1 t2 x,
+    typing_ctx C G t ((x ~ t1) ++ G') t2 ->
+    typing_ctx (ctx_abs t1 x C) G t G' (typ_arr t1 t2)
+| typing_ctx_app1 : forall C G G' t t2 t' e2,
+    typing_ctx C G t G' (typ_arr t2 t') ->
+    typing G' e2 t2 ->
+    typing_ctx (ctx_app1 C e2) G t G' t'
+| typing_ctx_app : forall C G G' t t2 t' e1,
+    typing G' e1 (typ_arr t2 t') ->
+    typing_ctx C G t G' t2  ->
+    typing_ctx (ctx_app2 e1 C) G t G' t'.
+
+Hint Constructors typing_ctx.
+
+
+(* The replacement operation preserves types *)
+Lemma typing_replace : forall C G t G' t' e,
+   typing_ctx C G t G' t' -> typing G e t -> typing G' (replace C e) t'.
+Proof.
+  intros C G t G' t' e H H1. 
+  induction H; simpl; auto.
+  - eapply (typing_rec_exists x);
+      autorewrite with lngen; auto. apply val_abs. (* lc *) admit.
+    eapply (typing_abs_exists y);
+      autorewrite with lngen; eauto.
+  - eapply (typing_rec_exists x);
+      autorewrite with lngen; auto. admit.
+    eapply (typing_abs_exists y);
+      autorewrite with lngen; eauto.
+  - eapply (typing_rec_exists x G' _ _ _ t');
+    autorewrite with lngen; auto. admit.
+    eapply (typing_abs_exists y);
+      autorewrite with lngen; eauto.
+  - eapply (typing_abs_exists x);
+      autorewrite with lngen; eauto.
+  - eapply typing_app; eauto.
+  - eapply typing_app; eauto.
+Admitted.
+
+(* Lemma 46.1 *)
+Lemma extension : forall G G' t t' C, typing_ctx C G t G' t' ->
+                                 exists G'', G = G'' ++ G'.
+Proof.
+  intros. induction H; auto.
+  - exists nil. simpl. auto.
+  - destruct IHtyping_ctx as [G'' EQ].
+    exists (G'' ++ (y ~ t') ++ (x ~ typ_nat)).
+    simpl_env. auto.
+  - destruct IHtyping_ctx as [G'' EQ].
+    exists (G'' ++ (x ~ t1)).
+    simpl_env. auto.
+Qed.
+
+
+(* Definition 46.4 *)
+
+Definition kleene_equivalence e1 e2 :=
+  exists v, value v /\ multistep e1 v /\ multistep e2 v.
+
+(* NOTE: Bob claims that this relation is clearly reflexive. But we can't 
+   prove that yet. *)
+
+Lemma kleene_sym  : forall e1 e2, kleene_equivalence e1 e2 -> kleene_equivalence e2 e1.
+Proof.
+  unfold kleene_equivalence.
+  intros.  destruct H as [v [V [M1 M2]]].
+  exists v. auto.
+Qed.
+
+Lemma kleene_trans : forall e1 e2 e3, kleene_equivalence e1 e2 -> kleene_equivalence e2 e3
+                                 -> kleene_equivalence e1 e3.
+Proof.
+  unfold kleene_equivalence.
+  intros.  destruct H as [v [V [M1 M2]]]. destruct H0 as [v' [V' [M1' M2']]].
+  exists v. split. auto. admit. (* derterminancy of evaluation *)
+Admitted.
+
+
+Definition observational_equivalence G e e' t :=
+  typing G e  t /\ typing G e' t /\
+  forall C, 
+    typing_ctx C G t nil typ_nat ->
+    kleene_equivalence (replace C e) (replace C e').
+
+(* We want to prove 46.6, but first we need a general definition of 
+   a "consistent congruence relation" *)
+
+Record open_equivalence (R : env -> exp -> exp -> typ -> Prop) := mkO
+{
+  (* Only holds for well-typed terms (with the same type) *)
+  open_typed : forall G e1 e2 t , R G e1 e2 t -> typing G e1 t /\ typing G e2 t;
+
+  (* Is an equivalence relation *)
+  open_refl : forall G e t, typing G e t -> R G e e t;
+  open_sym  : forall G e1 e2 t, R G e1 e2 t -> R G e2 e1 t;
+  open_trans : forall G e1 e2 e3 t, R G e1 e2 t -> R G e2 e3 t -> R G e1 e3 t;
+
+  (* Is consistent *)
+  open_consistent :  forall e1 e2,
+      R nil e1 e2 typ_nat -> kleene_equivalence e1 e2;
+
+  (* Is a congruence *)
+  open_congruence : forall G e e' t,
+      R G e e' t -> forall C G' t', typing_ctx C G t G' t'
+                              -> R G' (replace C e) (replace C e') t'
+}.
+
+(* Lemma 46.6 (first part). *)
+Lemma open_observational_notyet : open_equivalence observational_equivalence.
+Admitted.
+(* We can't actually prove this yet, because it relies on the 
+reflexivity of kleene_equivalence. *)
+
+(* However, we can prove everything else. *)
+Lemma  observational_typed :
+  forall G e1 e2 t , observational_equivalence G e1 e2 t -> typing G e1 t /\ typing G e2 t.
+Proof.
+  intros.  destruct H as [T1 [T2 CTX]]. auto.
+Qed.
+  
+  (* Is an equivalence relation *)
+Lemma observational_sym  : forall G e1 e2 t, observational_equivalence G e1 e2 t -> observational_equivalence G e2 e1 t.
+Proof.
+  unfold observational_equivalence.
+  intros. destruct H as [T1 [T2 CTX]].
+  repeat split; auto.
+  intros C CC.
+  apply kleene_sym. auto.
+Qed.
+
+Lemma observational_trans :
+  forall G e1 e2 e3 t, observational_equivalence G e1 e2 t
+                  -> observational_equivalence G e2 e3 t
+                  -> observational_equivalence G e1 e3 t.
+Proof.  
+  unfold observational_equivalence.
+  intros.
+  destruct H as [T1 [T2 CTX]].
+  destruct H0 as [T1' [T2' CTX']].
+  repeat split; auto.
+  intros C CC.
+  apply kleene_trans with (e2 := replace C e2). auto. auto.
+Qed.
+  
+  
+ (* Is consistent *)
+Lemma  observational_consistent :  forall e1 e2,
+    observational_equivalence nil e1 e2 typ_nat -> kleene_equivalence e1 e2.
+Proof.
+  unfold observational_equivalence.
+  intros.
+  destruct H as [T1 [T2 CTX]].
+  apply CTX with (C := ctx_top).
+  eapply typing_ctx_top.
+Qed.
+
+Fixpoint compose (C1 : ctx) (C2 : ctx) : ctx :=
+  match C1 with
+  | ctx_top => C2
+  | ctx_s C => ctx_s (compose C C2)
+  | ctx_rec1 C e1 x y t e2 => ctx_rec1 (compose C C2) e1 x y t e2
+  | ctx_rec2 e0 C x y t e2 => ctx_rec2 e0 (compose C C2) x y t e2
+  | ctx_rec3 e0 e1 x y t C => ctx_rec3 e0 e1 x y t (compose C C2)
+  | ctx_abs t x C => ctx_abs t x (compose C C2)
+  | ctx_app1 C e2 => ctx_app1 (compose C C2) e2
+  | ctx_app2 e1 C => ctx_app2 e1 (compose C C2)
+  end.
+
+Lemma replace_compose : forall C1 C2 e, replace C1 (replace C2 e) = replace (compose C1 C2) e.
+Proof.
+  intros C1. induction C1; intros; simpl; try rewrite IHC1; auto.
+Qed.
+
+(* Lemma 46.2 *)
+Lemma typing_compose : forall C1 C2 G t G' t' G'' t'',
+    typing_ctx C1 G t G' t' ->
+    typing_ctx C2 G' t' G'' t'' ->
+    typing_ctx (compose C2 C1) G t G'' t''.
+Proof.
+  intros. 
+  induction H0; intros; simpl; eauto.
+Qed.
+    
+  (* Is a congruence *)
+Lemma observational_congruence : forall G e e' t,
+    observational_equivalence G e e' t -> forall C G' t',
+      typing_ctx C G t G' t'
+      -> observational_equivalence G' (replace C e) (replace C e') t'.
+Proof.
+  intros.
+  unfold observational_equivalence.
+  destruct (observational_typed _ _ _ _ H) as [T1 T2].
+  repeat split. eapply typing_replace; eauto.
+  eapply typing_replace; eauto.
+  intros C' CT'.
+  rewrite replace_compose.
+  rewrite replace_compose.
+  destruct H as [Te [Te' CTX]].
+  eapply CTX.
+  eapply typing_compose; eauto.
+Qed.
+
+(* ------------ *)
+
+(* Lemma 46.6 *)
+(* Observational equivalence is the *largest* open_equivalence *)
+
+Lemma coarsest :
+  forall R G e1 e2 t,
+    open_equivalence R -> R G e1 e2 t -> observational_equivalence G e1 e2 t.
+Proof.
+  intros R G e1 e2 t OPEN H.
+  destruct (open_typed R OPEN _ _ _ _ H).
+  unfold observational_equivalence.
+  split. auto.
+  split. auto.
+  intros C CT.
+  pose (CONG := open_congruence R OPEN _ _ _ _ H C nil typ_nat CT).
+  clearbody CONG.
+  pose (CONS := open_consistent R OPEN _ _ CONG).
+  auto.
+Qed.  
+
+
+(*  ----------------- closing substitutions --------------------- *)
+
+Definition closing_subst := list (atom * exp).
+
+Inductive typing_cs : env -> closing_subst -> Prop :=
+| typing_cs_nil : typing_cs nil nil
+| typing_cs_cons : forall G g x t e,
+    typing nil e t ->
+    typing_cs G g ->
+    x `notin` dom G \u dom g ->
+    typing_cs ((x ~ t) ++ G) ((x ~ e) ++ g).
+
+Hint Constructors typing_cs.
+              
+Fixpoint apply_cs (g : closing_subst) (e : exp) : exp :=
+  match e with
+  | var_f y => match binds_lookup _ y g with
+              | inl (exist _ e0 _) => e0
+                    | inr _ => e
+                end
+  | s e1 => s (apply_cs g e1)
+  | app e1 e2 => app (apply_cs g e1) (apply_cs g e2)
+  | abs t e1 => abs t (apply_cs g e1)
+  | rec e0 e1 e2 => rec (apply_cs g e0) (apply_cs g e1) (apply_cs g e2)
+  | _ => e
+  end.
+
+  
+Inductive eq_cs (R : env -> exp -> exp -> typ -> Prop) : env -> closing_subst -> closing_subst -> Prop :=
+| eq_cs_nil  : eq_cs R nil nil nil
+| eq_cs_cons : forall G g1 g2 x t e1 e2,
+    eq_cs R G g1 g2 ->
+    R nil e1 e2 t ->
+    x `notin` dom g1 \u dom g2 \u dom G ->
+    eq_cs R ((x ~ t) ++ G) ((x ~ e1)++ g1) ((x ~ e2) ++ g2).
+
+Hint Constructors eq_cs.
+
+Lemma eq_cs_typing : forall G g1 g2,
+    eq_cs observational_equivalence G g1 g2 -> typing_cs G g1 /\ typing_cs G g2.
+Proof.                                
+  intro G. induction G; intros. inversion H. auto.
+  inversion H. subst.
+  destruct (observational_typed  _ _ _ _ H3).
+  destruct (IHG _ _ H2).
+  split. econstructor; eauto.
+  econstructor; eauto.
+Qed.      
+
+(* -----   Lemma 46.7 -------  *)
+
+Lemma apply_nil : forall e, apply_cs nil e = e.
+Proof.
+  induction e; simpl; try rewrite IHe; auto.
+  rewrite IHe1. rewrite IHe2. rewrite IHe3. auto.
+  rewrite IHe1. rewrite IHe2. auto.
+Qed.  
+
+Lemma apply_cons : forall x e1 g e,
+    x `notin` dom g -> apply_cs ((x ~ e1) ++ g) e = apply_cs g (subst_exp e1 x e).
+Proof.
+  intros.
+  induction e; simpl; auto.
+  - destruct (KeySetFacts.eq_dec x0 x).
+    + subst.
+      destruct (binds_lookup exp x g). destruct s.
+      apply binds_In in b. contradiction.
+      simpl. admit.
+    + destruct (binds_lookup exp x0 g). destruct s.
+      admit.
+      simpl. destruct (x0 == x). contradiction. admit.
+  - simpl in IHe. rewrite IHe. auto.
+  - simpl in *. rewrite IHe1. rewrite IHe2. rewrite IHe3. auto.
+Admitted.
+
+
+Lemma apply_cs_typing : forall G g, typing_cs G g -> forall e t, typing G e t -> typing nil (apply_cs g e) t.
+Proof.
+  intros G g H. induction H.
+  intros. rewrite apply_nil. auto.
+  intros.
+  pose (K := typing_uniq _ _ _ H2). inversion K. subst. clear K.
+  rewrite apply_cons.
+  apply IHtyping_cs.
+  eapply typing_subst_simple. eauto.
+  eapply typing_weakening with (F := G)(E:=nil) in H.
+  rewrite app_nil_r in H. auto.
+  rewrite app_nil_r. auto. auto.
+Qed.  
+  
+(* Closing substitutions close terms. *)
+Lemma closing_typed : forall G g, typing_cs G g -> 
+    forall e e' t, observational_equivalence G e e' t -> 
+    observational_equivalence nil (apply_cs g e) (apply_cs g e') t.
+Proof.
+  intros.  unfold observational_equivalence in *.
+  destruct H0 as [T1 [T2 CT]].
+  split. eapply apply_cs_typing. eauto. eauto.
+  split. eapply apply_cs_typing. eauto. eauto.
+  intros C CTX.
+Admitted.
+
+Lemma closed_context : forall C g t,
+    typing_ctx C nil t nil typ_nat -> forall G, typing_cs G g ->
+    forall e, replace C (apply_cs g e) = apply_cs g (replace C e).
+Proof.
+  intros C. induction C; intros;  simpl; auto.
+  - inversion H.
+    erewrite IHC; eauto.
+  - inversion H.
+    erewrite IHC; eauto.
+    admit.
+Admitted.
+
+(*
+Fixpoint make_ctx (G : env)(g : closing_subst)(C : ctx) : ctx :=
+  match G with
+  | nil => ctx_top
+  | cons (x,t) G' => ctx_abs t x (make_ctx G' g (ctx_app1 C (apply_cs g (var_f x))))
+  end.
+
+Lemma typing_make_ctx :
+  forall G g, typing_ctx C G t G typ_nat ->
+         typing_ctx (make_ctx G g C) G t nil typ_nat
+*)
+
+Lemma closing_eq : forall G e e' t g g',
+    observational_equivalence G e e' t -> eq_cs observational_equivalence G g g' ->
+    observational_equivalence nil (apply_cs g e) (apply_cs g' e') t.
+Proof.
+  intros.
+  unfold observational_equivalence.
+  destruct (observational_typed _ _ _ _ H) as [h0 h1].
+  destruct (eq_cs_typing _ _ _ H0) as [Tg Tg'].
+  split. apply apply_cs_typing with (G := G); eauto. 
+  split. apply apply_cs_typing with (G := G); eauto. 
+  intros C CT.
+  rewrite closed_context with (t := t)(G := G); auto.
+  rewrite closed_context with (t := t)(G := G); auto.
+Admitted.
+
+(* --------------------- 46.2 Logical equivalence -------------------------- *)
+
+Fixpoint logical_equivalence (e e' : exp) (t : typ) {struct t} : Prop :=
+  match t with
+  | typ_nat => typing nil e typ_nat /\ typing nil e' typ_nat /\ kleene_equivalence e e' 
+  | typ_arr t1 t2 =>
+    typing nil e (typ_arr t1 t2) /\ typing nil e' (typ_arr t1 t2) /\
+    forall e1 e1', logical_equivalence e1 e1' t1 ->
+              logical_equivalence (app e e1) (app e' e1') t2
+  end.
+
+
+(* ------------------ proof by nat-induction --------------------- *)
+
+Fixpoint from_nat (n : nat) : exp :=
+  match n with
+  | O => z
+  | S n => s (from_nat n)
+  end.
+
+Inductive as_nat : nat -> exp -> Prop :=
+| as_nat_z : as_nat O z
+| as_nat_s : forall n e, as_nat n e -> as_nat (S n) (s e).
+Hint Constructors as_nat.
+
+Lemma to_nat : forall e, value e -> typing nil e typ_nat -> exists n, as_nat n e.
+Proof. 
+  intros e V. induction V; intros.
+  inversion H. exists O. auto.
+  inversion H.
+  destruct (IHV H2) as [m A].
+  exists (S m). auto.
+  inversion H0.
+Qed.
+
+Lemma as_from_nat : forall n, as_nat n (from_nat n).
+Proof. induction n.
+       simpl. auto.
+       simpl in *. auto.
+Qed.
+
+Lemma nat_induction : forall e e', logical_equivalence e e' typ_nat
+                              -> forall (R : exp -> exp -> Prop), R z z -> (forall v, value v -> R v v -> R (s v) (s v)) -> R e e'.
+Proof.                                  
+  intros.
+  unfold logical_equivalence in H.
+  unfold kleene_equivalence in H.
+  destruct H as [T1 [T2 [v [VV [Se Se']]]]].
+  destruct (to_nat v VV). admit.
+  generalize dependent e. generalize dependent e'. generalize dependent v. induction x.
+  - intros. inversion H. subst.  (* Need to know that R is closed under reverse_evaluation *)
+    admit.
+  - intros. inversion H. subst.
+    assert (R (s e0) (s e0) -> R e e'). admit.
+    apply H2. apply H1. inversion VV. auto.
+    inversion VV.
+    apply (IHx e0); eauto. admit. admit. admit. admit.
+Admitted.
+
+(* ------------------ sym & trans --------------------- *)
+
+Lemma logical_typing : forall t e e',
+    logical_equivalence e e' t -> typing nil e t /\ typing nil e' t.
+Proof.
+  induction t; intros; simpl in *.
+  destruct H as [H1 [H2 _]]. auto.
+  destruct H as [H1 [H2 G3]].
+  auto.
+Qed.  
+
+(* Lemma 46.9 *)
+Lemma logical_sym : forall e e' t,
+    logical_equivalence e e' t -> logical_equivalence e' e t.
+Admitted.
+
+Lemma logical_trans : forall e e' e'' t,
+    logical_equivalence e e' t ->
+    logical_equivalence e' e'' t ->
+    logical_equivalence e e'' t.
+Admitted.
+
+
+(* -------------- extension to open terms --------------------- *)
+
+Definition open_logical_equivalence G e e' t :=
+  typing G e t /\
+  typing G e' t /\
+  forall g g', eq_cs (fun G => logical_equivalence) G g g' ->
+          logical_equivalence (apply_cs g e) (apply_cs g' e') t.
+
+Lemma open_logical_sym : forall G e e' t,
+    open_logical_equivalence G e e' t -> open_logical_equivalence G e' e t.
+Admitted.
+
+Lemma open_logical_trans : forall G e e' e'' t,
+    open_logical_equivalence G e e' t ->
+    open_logical_equivalence G e' e'' t ->
+    open_logical_equivalence G e e'' t.
+Admitted.
+
+(* -------------------------- 46.3 ---------------------------- *)
+
+Lemma converse_evaluation_logical : forall e e' t,
+    logical_equivalence e e' t -> forall d, eval e e -> logical_equivalence d e' t.
+Proof.
+  intros e e' t. induction t.
+  - intros.
+    unfold logical_equivalence in *. unfold kleene_equivalence in *.
+    admit.
+  - intros.
+    simpl in *.
+    admit.
+Admitted.
+
+
+Lemma consistency_logical : forall e e', logical_equivalence e e' typ_nat -> kleene_equivalence e e'.
+Proof.
+  unfold logical_equivalence.
+  intros. destruct H as [h0 [h1 h2]].
+  auto.
+Qed.
+
+
+Lemma open_logical_refl : forall G e t, typing G e t -> open_logical_equivalence G e e t.
+Proof.
+  intros G e t H.
+  induction H; unfold open_logical_equivalence;
+    split; eauto; split; eauto; intros g g' EQ.
+  - admit.
+  - simpl. split. auto. split. auto.
+    unfold kleene_equivalence. exists z. split. auto. split. admit. admit.
+  - admit.
+Admitted.
+
+Lemma termination : forall e, typing nil e typ_nat -> exists v, multistep e v /\ value v.
+Proof.
+  intros e H.
+  apply open_logical_refl in H.
+  unfold open_logical_equivalence in H.
+  destruct H as [_ [_ H0]].
+  destruct (H0 nil nil) as [k0 [k1 k2]].
+  apply eq_cs_nil.
+  unfold kleene_equivalence in k2.
+  destruct k2 as [v [VV [Ms1 Ms2]]].
+  exists v. simpl in *. split. rewrite apply_nil in Ms1.  auto.
+  auto.
+Qed.
+
+(* This wasn't obvious before, but it is provable now. *)
+Lemma kleene_refl : forall e, typing nil e typ_nat -> kleene_equivalence e e.
+Proof.
+  intros e H.
+  apply termination in H.
+  unfold kleene_equivalence.
+  destruct H as [v [MS V]].
+  exists v. auto.
+Qed.
+
+Lemma open_observational : open_equivalence observational_equivalence.
+  apply mkO.
+  - apply observational_typed. 
+  - intros. unfold observational_equivalence.
+    split. auto. split. auto. intros.
+    apply kleene_refl.
+    apply typing_replace with (G := G) (t:=t). auto. auto.
+  - apply observational_sym.
+  - apply observational_trans.
+  - apply observational_consistent.
+  - apply observational_congruence. 
+Qed.
+
+(* Lemma 46.16 *)
+Lemma open_logical_congruence :
+  forall C0 G t G0 t0,
+    typing_ctx C0 G t G0 t0 ->
+    forall e e', open_logical_equivalence G e e' t ->
+            open_logical_equivalence G0 (replace C0 e) (replace C0 e') t0.
+Proof.
+  intros C0 G t G0 t0 H. induction H; intros; simpl; auto.
+  - unfold open_logical_equivalence in *.
+    destruct H0 as [Te [Te' LL]].
+    split. econstructor. eapply typing_replace; eauto.
+    split. econstructor. eapply typing_replace; eauto.
+    intros g g' EQ.
+    simpl.
+    split. econstructor. eapply apply_cs_typing with (G := G').
+    admit. eapply typing_replace; eauto.  (* equal cs are typed. *)
+    split. econstructor. eapply apply_cs_typing.
+    admit. eapply typing_replace; eauto.
+    destruct (IHtyping_ctx e e') as [k0 [k1 FF]].
+    repeat split.  auto. auto. auto.
+    destruct (FF g g') as [h0 [h1 GG]]. auto.
+    unfold kleene_equivalence in *.
+    destruct GG as [v [MS1 MS2]].
+    exists (s v). split. auto.
+    split. admit. admit. (* multistep is a congruence *)
+Admitted.
+    
+Lemma open_logical : open_equivalence open_logical_equivalence.
+Proof.
+  apply mkO.
+  - intros. unfold open_logical_equivalence in H.
+    destruct H as [T1 [T2 _]]. auto.
+  - apply open_logical_refl.
+  - apply open_logical_sym.
+  - apply open_logical_trans.
+  - (* consistent *) intros.
+    destruct H as [T1 [T2 C]].
+    destruct (C nil nil) as [h0 [h1 k]]. eauto.
+    rewrite apply_nil in k.
+    rewrite apply_nil in k.
+    auto.
+  - (* congruent *)
+    intros.
+    eapply open_logical_congruence; eauto.
+Qed.
+
+(* Theorem 46.17 *)
+(* Logical equivalence implies observational equivalence. *)
+Lemma logical_is_observational : forall G e e' t,
+    open_logical_equivalence G e e' t ->
+    observational_equivalence G e e' t.
+Proof.
+  intros.
+  eapply coarsest.
+  eapply open_logical. auto.
+Qed.
+
+(* Lemma 46.19 *)
+Lemma closed_observational_is_logical : forall t e e', 
+    observational_equivalence nil e e' t -> logical_equivalence e e' t.
+Proof.
+  induction t.
+  - intros. unfold logical_equivalence, observational_equivalence in *.
+    destruct H as [T1 [T2 CT]].
+    split. auto. split. auto.
+    pose (K := CT ctx_top (@typing_ctx_top nil typ_nat)).
+    simpl in K. auto.
+  - intros.
+    pose (M := H).
+    destruct M as [T1 [T2 CT]].
+    split. auto. split. auto.
+    intros e1 e1' Le1.
+    destruct (logical_typing _ _ _ Le1) as [U1 U2].
+    assert (observational_equivalence nil e1 e1' t1).
+    { eapply logical_is_observational.
+      unfold open_logical_equivalence.
+      split. auto. split. auto.
+      intros. inversion H0. subst.
+      rewrite apply_nil.
+      rewrite apply_nil.
+      auto. }
+    assert (observational_equivalence nil (app e e1) (app e' e1') t2).
+    { eapply observational_trans with (e2 := app e e1').
+      replace (app e e1) with (replace (ctx_app2 e ctx_top) e1); auto.
+      replace (app e e1') with (replace (ctx_app2 e ctx_top) e1'); auto.
+      eapply observational_congruence. eauto.
+      eauto.
+      replace (app e e1') with (replace (ctx_app1 ctx_top e1') e); auto.
+      replace (app e' e1') with (replace (ctx_app1 ctx_top e1') e'); auto.
+      eapply observational_congruence. eauto.
+      eauto. }
+    eauto.
+Qed.    
+    
+(* Lemma 46.19 *)
+Lemma observational_is_logical : forall G e e' t, 
+    observational_equivalence G e e' t -> open_logical_equivalence G e e' t.
+Proof.
+  intros.
+  unfold open_logical_equivalence.
+  destruct (observational_typed _ _ _ _ H) as [T1 T2].
+  split. auto.
+  split. auto.
+  intros g g' EQg.
+  apply closed_observational_is_logical.
+  apply closing_eq with (G := G). auto.
+  admit. (* map Lemma 46.19 *)
+Admitted.
